src/refinement/AlgorithmicPF_Algorithmic.v
@@ -31,8 +31,8 @@ Lemma lift_machine_state_step
       (STEP2: rtc (Machine.step ExecUnit.state_step) m2 m3)
       (NOPROMISE: Machine.no_promise m3):
   AMachine.step ExecUnit.state_step
-                (AMachine.mk m1 (IdMap.map (fun _ => Lock.init) m1.(Machine.tpool)))
-                (AMachine.mk m2 (IdMap.map (fun _ => Lock.init) m2.(Machine.tpool))).
+                (AMachine.mk m1 (fun tid => option_map (fun _ => Lock.init) (IdMap.find tid m1.(Machine.tpool))))
+                (AMachine.mk m2 (fun tid => option_map (fun _ => Lock.init) (IdMap.find tid m2.(Machine.tpool)))).
 Proof.
   inv STEP1. econs; eauto; ss.
 Admitted.
@@ -43,8 +43,8 @@ Lemma lift_rtc_machine_state_step
       (STEP2: rtc (Machine.step ExecUnit.state_step) m2 m3)
       (NOPROMISE: Machine.no_promise m3):
   rtc (AMachine.step ExecUnit.state_step)
-      (AMachine.mk m1 (IdMap.map (fun _ => Lock.init) m1.(Machine.tpool)))
-      (AMachine.mk m2 (IdMap.map (fun _ => Lock.init) m2.(Machine.tpool))).
+      (AMachine.mk m1 (fun tid => option_map (fun _ => Lock.init) (IdMap.find tid m1.(Machine.tpool))))
+      (AMachine.mk m2 (fun tid => option_map (fun _ => Lock.init) (IdMap.find tid m2.(Machine.tpool)))).
 Proof.
   revert STEP2 NOPROMISE. induction STEP1; eauto. i.
   exploit lift_machine_state_step; try exact NOPROMISE; eauto. etrans; eauto.
@@ -57,16 +57,19 @@ Theorem algorithmic_pf_to_algorithmic
     <<EXEC: AMachine.exec p m'>> /\
     <<EQUIV: Machine.equiv m m'>>.
 Proof.
-  (* TODO: do it first.  change the lock type to function. *)
-  inv EXEC. exploit state_exec_rtc_state_step; eauto. i. des.
-  exploit Machine.equiv_no_promise; eauto. i.
-  destruct am1. ss.
-  assert (tlocks = IdMap.map (fun _ => Lock.init) machine.(Machine.tpool)) by admit. subst. ss.
-  exploit lift_rtc_machine_state_step; try exact x0; eauto. i.
-  eexists (AMachine.mk m2' _). splits; eauto. econs.
-  - etrans.
-    + eapply rtc_mon; [|by eauto]. apply AMachine.step_mon. right. ss.
-    + eapply rtc_mon; [|by eauto]. apply AMachine.step_mon. left. ss.
-  - ss.
-  - ss.
+(*   inv EXEC. exploit state_exec_rtc_state_step; eauto. i. des. *)
+(*   exploit Machine.equiv_no_promise; eauto. i. *)
+(*   destruct am1. ss. *)
+(*   assert (tlocks = (fun tid => option_map (fun _ => Lock.init) (IdMap.find tid machine.(Machine.tpool)))). *)
+(*   { funext. i.  *)
+
+(* IdMap.map (fun _ => Lock.init) machine.(Machine.tpool)). *)
+(*     by admit. subst. ss. *)
+(*   exploit lift_rtc_machine_state_step; try exact x0; eauto. i. *)
+(*   eexists (AMachine.mk m2' _). splits; eauto. econs. *)
+(*   - etrans. *)
+(*     + eapply rtc_mon; [|by eauto]. apply AMachine.step_mon. right. ss. *)
+(*     + eapply rtc_mon; [|by eauto]. apply AMachine.step_mon. left. ss. *)
+(*   - ss. *)
+(*   - ss. *)
 Admitted.
